progs/verif_even.v
@@ -38,7 +38,7 @@ Qed.
 Definition odd_spec :=
  DECLARE _odd
   WITH z : Z, v : val
-  PRE [ (*_n*) 1%positive OF tuint] PROP(repr z v) LOCAL(`(eq v) (eval_id (*_n*) 1%positive)) SEP()
+  PRE [ _n (*1%positive*) OF tuint] PROP(repr z v) LOCAL(`(eq v) (eval_id _n (*1%positive*))) SEP()
   POST [ tint ] 
     PROP() LOCAL(`(eq (Vint (if Z.odd z then Int.one else Int.zero))) retval) SEP().
 
@@ -68,11 +68,10 @@ forward_if (PROP (repr z v /\ z > 0) LOCAL (`(eq v) (eval_id _n)) SEP ()).
 * forward; eapply repr0_even in H0; eauto; rewrite H0; entailer.
 * forward; entailer; inv H.
   assert (z <> 0) by (apply repr_eq0_not0; auto). entailer.
-* forward_call (z-1,Vint (Int.sub (Int.repr z) (Int.repr 1))). 
+* forward_call (z-1,Vint (Int.sub (Int.repr z) (Int.repr 1))).
   entailer; inversion H; subst z0; rewrite <-H5 in H2; inversion H2; subst n.
-  assert (repr (z - 1) (Vint (Int.repr (z - 1)))). 
-  { clear -H H1. inv H. constructor. omega. }
   entailer!.
+  inv H. constructor. omega.
   after_call; forward.
   rewrite Z.odd_sub; simpl. 
   case_eq (Z.odd z); rewrite Zodd_even_bool; destruct (Z.even z); simpl; try congruence.
@@ -96,12 +95,15 @@ Lemma all_funcs_correct: semax_func Vprog Gprog (prog_funct prog) Gprog.
 Proof.
 unfold Gprog, prog, prog_funct.
 semax_func_skipn.
-apply semax_func_cons_ext; auto.
-set (sig := ((1%positive,tuint):: nil, tint)).
-eapply (semax_ext NullExtension.Espec _odd sig (Z*val)).
+eapply semax_func_cons_ext; try reflexivity.
+intros [? ?] ?. normalize. entailer!.
+destruct ret; unfold retval, eval_id in H; simpl in H; subst; hnf; auto; discriminate.
+admit.
+(*eapply (semax_ext Espec _odd _(Z*val)).
 { left; auto. }
 { split; simpl; auto. intros C. destruct C; auto. inv H; auto. inv H; auto. inv H0.
 split; auto. intros C. inv C; auto. inv H. }
+*)
 semax_func_cons body_even.
 semax_func_cons body_main.
 apply semax_func_nil.
